Abelianization of the modular group PSL(2,Z).

Adapted from TypeTopology, `Groups.ModularGroup.Abelianization`
(Todd Waugh Ambridge). This module defines the abelianization map
`ab : PSL2Z â†’ Bool Ã— ğŸ›` and proves it is a surjective homomorphism
with respect to the group structures on PSL2Z and the product of
cyclic groups Z/2 Ã— Z/3.

```agda
{-# OPTIONS --safe --erased-cubical --no-guardedness --no-sized-types #-}

module Lib.Group.Modular.Abelianization where

open import Core.Base using (_â‰¡_; refl; sym; ap; ap2)
open import Core.Kan using (_âˆ™_)
open import Core.Type using (Type; 0â„“; âŠ¤; tt)
open import Core.Data.Sigma using (Î£; _,_; fst; snd; _Ã—_)
open import Core.Data.Sum using (_âŠ_; inl; inr)
open import Core.Data.Bool using (Bool; true; false)
open import Core.Data.Empty using (âŠ¥; ex-falso)
open import Core.Path using (_â‰¢_)
open import Core.Transport.J using (subst)

open import Lib.Group.Modular.Multiplication
open import Lib.Group.Modular.Properties
open import Lib.Group.Modular.Base
open import Lib.Group.Modular.Type

private
  _â‰¡âŸ¨_âŸ©_ : âˆ€ {â„“} {A : Type â„“} (x : A) {y z : A}
          â†’ x â‰¡ y â†’ y â‰¡ z â†’ x â‰¡ z
  x â‰¡âŸ¨ p âŸ© q = p âˆ™ q

  _âˆ : âˆ€ {â„“} {A : Type â„“} (x : A) â†’ x â‰¡ x
  x âˆ = refl

  infixr 2 _â‰¡âŸ¨_âŸ©_
  infix  3 _âˆ
```


## The three-element type

The cyclic group Z/3 represented as a three-element sum type.

```agda
ğŸ› : Type 0â„“
ğŸ› = âŠ¤ âŠ âŠ¤ âŠ âŠ¤

pattern ğŸ¬ = inl tt
pattern ğŸ­ = inr (inl tt)
pattern ğŸ® = inr (inr tt)
```


## Modular arithmetic

Addition mod 3 and mod 2, defined by exhaustive case split.

```agda
_+â‚ƒ_ : ğŸ› â†’ ğŸ› â†’ ğŸ›
ğŸ¬ +â‚ƒ y = y
ğŸ­ +â‚ƒ ğŸ¬ = ğŸ­
ğŸ­ +â‚ƒ ğŸ­ = ğŸ®
ğŸ­ +â‚ƒ ğŸ® = ğŸ¬
ğŸ® +â‚ƒ ğŸ¬ = ğŸ®
ğŸ® +â‚ƒ ğŸ­ = ğŸ¬
ğŸ® +â‚ƒ ğŸ® = ğŸ­

_+â‚‚_ : Bool â†’ Bool â†’ Bool
false +â‚‚ y = y
true  +â‚‚ false = true
true  +â‚‚ true  = false
```


## Arithmetic lemmas

All proved by exhaustive case split; every case is `refl`.

```agda
+â‚‚-comm : (x y : Bool) â†’ x +â‚‚ y â‰¡ y +â‚‚ x
+â‚‚-comm false false = refl
+â‚‚-comm false true  = refl
+â‚‚-comm true  false = refl
+â‚‚-comm true  true  = refl

+â‚‚-assoc : (x y z : Bool) â†’ (x +â‚‚ y) +â‚‚ z â‰¡ x +â‚‚ (y +â‚‚ z)
+â‚‚-assoc false y     z     = refl
+â‚‚-assoc true  false z     = refl
+â‚‚-assoc true  true  false = refl
+â‚‚-assoc true  true  true  = refl

+â‚‚-unit-right : (x : Bool) â†’ x +â‚‚ false â‰¡ x
+â‚‚-unit-right false = refl
+â‚‚-unit-right true  = refl

+â‚‚-cancel : (x : Bool) â†’ x +â‚‚ x â‰¡ false
+â‚‚-cancel false = refl
+â‚‚-cancel true  = refl

+â‚‚-cancel-inv : (x : Bool) â†’ true +â‚‚ (true +â‚‚ x) â‰¡ x
+â‚‚-cancel-inv false = refl
+â‚‚-cancel-inv true  = refl

+â‚ƒ-comm : (x y : ğŸ›) â†’ x +â‚ƒ y â‰¡ y +â‚ƒ x
+â‚ƒ-comm ğŸ¬ ğŸ¬ = refl
+â‚ƒ-comm ğŸ¬ ğŸ­ = refl
+â‚ƒ-comm ğŸ¬ ğŸ® = refl
+â‚ƒ-comm ğŸ­ ğŸ¬ = refl
+â‚ƒ-comm ğŸ­ ğŸ­ = refl
+â‚ƒ-comm ğŸ­ ğŸ® = refl
+â‚ƒ-comm ğŸ® ğŸ¬ = refl
+â‚ƒ-comm ğŸ® ğŸ­ = refl
+â‚ƒ-comm ğŸ® ğŸ® = refl

+â‚ƒ-assoc : (x y z : ğŸ›) â†’ (x +â‚ƒ y) +â‚ƒ z â‰¡ x +â‚ƒ (y +â‚ƒ z)
+â‚ƒ-assoc ğŸ¬ y z = refl
+â‚ƒ-assoc ğŸ­ ğŸ¬ z = refl
+â‚ƒ-assoc ğŸ­ ğŸ­ ğŸ¬ = refl
+â‚ƒ-assoc ğŸ­ ğŸ­ ğŸ­ = refl
+â‚ƒ-assoc ğŸ­ ğŸ­ ğŸ® = refl
+â‚ƒ-assoc ğŸ­ ğŸ® ğŸ¬ = refl
+â‚ƒ-assoc ğŸ­ ğŸ® ğŸ­ = refl
+â‚ƒ-assoc ğŸ­ ğŸ® ğŸ® = refl
+â‚ƒ-assoc ğŸ® ğŸ¬ z = refl
+â‚ƒ-assoc ğŸ® ğŸ­ ğŸ¬ = refl
+â‚ƒ-assoc ğŸ® ğŸ­ ğŸ­ = refl
+â‚ƒ-assoc ğŸ® ğŸ­ ğŸ® = refl
+â‚ƒ-assoc ğŸ® ğŸ® ğŸ¬ = refl
+â‚ƒ-assoc ğŸ® ğŸ® ğŸ­ = refl
+â‚ƒ-assoc ğŸ® ğŸ® ğŸ® = refl

+â‚ƒ-unit-right : (x : ğŸ›) â†’ x +â‚ƒ ğŸ¬ â‰¡ x
+â‚ƒ-unit-right ğŸ¬ = refl
+â‚ƒ-unit-right ğŸ­ = refl
+â‚ƒ-unit-right ğŸ® = refl
```


## The abelianization type

The target group is the product Z/2 Ã— Z/3 with componentwise
addition.

```agda
Ab : Type 0â„“
Ab = Bool Ã— ğŸ›

_+á´¬_ : Ab â†’ Ab â†’ Ab
(sâ‚ , râ‚) +á´¬ (sâ‚‚ , râ‚‚) = (sâ‚ +â‚‚ sâ‚‚) , (râ‚ +â‚ƒ râ‚‚)

0á´¬ : Ab
0á´¬ = false , ğŸ¬
```


## Abelian group laws for Ab

```agda
+á´¬-comm : (a b : Ab) â†’ a +á´¬ b â‰¡ b +á´¬ a
+á´¬-comm (sâ‚ , râ‚) (sâ‚‚ , râ‚‚) =
  ap2 _,_ (+â‚‚-comm sâ‚ sâ‚‚) (+â‚ƒ-comm râ‚ râ‚‚)

+á´¬-assoc : (a b c : Ab) â†’ (a +á´¬ b) +á´¬ c â‰¡ a +á´¬ (b +á´¬ c)
+á´¬-assoc (sâ‚ , râ‚) (sâ‚‚ , râ‚‚) (sâ‚ƒ , râ‚ƒ) =
  ap2 _,_ (+â‚‚-assoc sâ‚ sâ‚‚ sâ‚ƒ) (+â‚ƒ-assoc râ‚ râ‚‚ râ‚ƒ)

+á´¬-unit-right : (a : Ab) â†’ a +á´¬ 0á´¬ â‰¡ a
+á´¬-unit-right (sâ‚ , râ‚) =
  ap2 _,_ (+â‚‚-unit-right sâ‚) (+â‚ƒ-unit-right râ‚)
```


## The abelianization map

Defined by mutual recursion on S-edges and R-edges.

```agda
ab-Î· : S-edge â†’ Ab
ab-Î¸ : R-edge â†’ Ab

ab-Î· eâ‚€         = false , ğŸ¬
ab-Î· eâ‚         = true , ğŸ¬
ab-Î· (cross re) =
  (true +â‚‚ fst (ab-Î¸ re)) , snd (ab-Î¸ re)

ab-Î¸ (r+ se) =
  fst (ab-Î· se) , (ğŸ­ +â‚ƒ snd (ab-Î· se))
ab-Î¸ (r- se) =
  fst (ab-Î· se) , (ğŸ® +â‚ƒ snd (ab-Î· se))

ab : PSL2Z â†’ Ab
ab (Î· se) = ab-Î· se
ab (Î¸ re) = ab-Î¸ re
```


## Generator interaction lemmas

How the abelianization map interacts with the generators s, r, and
r-squared.

```agda
ab-s : (x : PSL2Z) â†’ ab (s x) â‰¡ (true , ğŸ¬) +á´¬ ab x
ab-s (Î· eâ‚€)         = refl
ab-s (Î· eâ‚)         = refl
ab-s (Î· (cross re)) =
  sym (ap2 _,_ (+â‚‚-cancel-inv (fst (ab-Î¸ re))) refl)
ab-s (Î¸ re)          = refl

ab-r : (x : PSL2Z) â†’ ab (r x) â‰¡ (false , ğŸ­) +á´¬ ab x
ab-r (Î· eâ‚€)         = refl
ab-r (Î· eâ‚)         = refl
ab-r (Î· (cross re)) = refl
ab-r (Î¸ (r+ se))    =
  ap2 _,_ refl (+â‚ƒ-assoc ğŸ­ ğŸ­ (snd (ab-Î· se)))
ab-r (Î¸ (r- se))    =
  ap2 _,_ refl (+â‚ƒ-assoc ğŸ­ ğŸ® (snd (ab-Î· se)))
```

The r-squared case derives from two applications of `ab-r`.

```agda
ab-rÂ² : (x : PSL2Z) â†’ ab (rÂ² x) â‰¡ (false , ğŸ®) +á´¬ ab x
ab-rÂ² x =
  ab-r (r x)
  âˆ™ ap ((false , ğŸ­) +á´¬_) (ab-r x)
  âˆ™ sym (+á´¬-assoc (false , ğŸ­) (false , ğŸ­) (ab x))
```


## Key structural lemmas

Right-addition lemmas for the abelianization of R-edges.

```agda
ab-Î·+R : (se : S-edge) â†’ ab-Î· se +á´¬ (false , ğŸ­) â‰¡ ab-Î¸ (r+ se)
ab-Î·+R se =
  ap2 _,_ (+â‚‚-unit-right (fst (ab-Î· se)))
           (+â‚ƒ-comm (snd (ab-Î· se)) ğŸ­)

ab-Î·+RÂ² : (se : S-edge) â†’ ab-Î· se +á´¬ (false , ğŸ®) â‰¡ ab-Î¸ (r- se)
ab-Î·+RÂ² se =
  ap2 _,_ (+â‚‚-unit-right (fst (ab-Î· se)))
           (+â‚ƒ-comm (snd (ab-Î· se)) ğŸ®)
```


## The homomorphism proof

The abelianization map preserves multiplication.

```agda
ab-hom : (x y : PSL2Z) â†’ ab (x Â· y) â‰¡ ab x +á´¬ ab y
ab-hom (Î· eâ‚€) y = refl
ab-hom (Î· eâ‚) y = ab-s y
ab-hom (Î· (cross re)) y =
  ab ((sâˆ™ re) Â· y)
    â‰¡âŸ¨ ap ab (Â·-s-left (Î¸ re) y) âŸ©
  ab (s ((Î¸ re) Â· y))
    â‰¡âŸ¨ ab-s ((Î¸ re) Â· y) âŸ©
  (true , ğŸ¬) +á´¬ ab ((Î¸ re) Â· y)
    â‰¡âŸ¨ ap ((true , ğŸ¬) +á´¬_) (ab-hom (Î¸ re) y) âŸ©
  (true , ğŸ¬) +á´¬ (ab-Î¸ re +á´¬ ab y)
    â‰¡âŸ¨ sym (+á´¬-assoc (true , ğŸ¬) (ab-Î¸ re) (ab y)) âŸ©
  ((true , ğŸ¬) +á´¬ ab-Î¸ re) +á´¬ ab y
    âˆ
ab-hom (Î¸ (r+ se)) y =
  ab ((râˆ™ se) Â· y)
    â‰¡âŸ¨ ap (Î» z â†’ ab (z Â· y)) (sym (r-Î· se)) âŸ©
  ab ((r (Î· se)) Â· y)
    â‰¡âŸ¨ ap ab (Â·-r-left (Î· se) y) âŸ©
  ab (r ((Î· se) Â· y))
    â‰¡âŸ¨ ab-r ((Î· se) Â· y) âŸ©
  (false , ğŸ­) +á´¬ ab ((Î· se) Â· y)
    â‰¡âŸ¨ ap ((false , ğŸ­) +á´¬_) (ab-hom (Î· se) y) âŸ©
  (false , ğŸ­) +á´¬ (ab-Î· se +á´¬ ab y)
    â‰¡âŸ¨ sym (+á´¬-assoc (false , ğŸ­) (ab-Î· se) (ab y)) âŸ©
  ((false , ğŸ­) +á´¬ ab-Î· se) +á´¬ ab y
    â‰¡âŸ¨ ap (_+á´¬ ab y) (+á´¬-comm (false , ğŸ­) (ab-Î· se)) âŸ©
  (ab-Î· se +á´¬ (false , ğŸ­)) +á´¬ ab y
    â‰¡âŸ¨ ap (_+á´¬ ab y) (ab-Î·+R se) âŸ©
  ab-Î¸ (r+ se) +á´¬ ab y
    âˆ
ab-hom (Î¸ (r- se)) y =
  ab ((rÂ²âˆ™ se) Â· y)
    â‰¡âŸ¨ ap (Î» z â†’ ab (z Â· y)) (sym (rÂ²-Î· se)) âŸ©
  ab ((rÂ² (Î· se)) Â· y)
    â‰¡âŸ¨ ap ab (Â·-rÂ²-left (Î· se) y) âŸ©
  ab (rÂ² ((Î· se) Â· y))
    â‰¡âŸ¨ ab-rÂ² ((Î· se) Â· y) âŸ©
  (false , ğŸ®) +á´¬ ab ((Î· se) Â· y)
    â‰¡âŸ¨ ap ((false , ğŸ®) +á´¬_) (ab-hom (Î· se) y) âŸ©
  (false , ğŸ®) +á´¬ (ab-Î· se +á´¬ ab y)
    â‰¡âŸ¨ sym (+á´¬-assoc (false , ğŸ®) (ab-Î· se) (ab y)) âŸ©
  ((false , ğŸ®) +á´¬ ab-Î· se) +á´¬ ab y
    â‰¡âŸ¨ ap (_+á´¬ ab y) (+á´¬-comm (false , ğŸ®) (ab-Î· se)) âŸ©
  (ab-Î· se +á´¬ (false , ğŸ®)) +á´¬ ab y
    â‰¡âŸ¨ ap (_+á´¬ ab y) (ab-Î·+RÂ² se) âŸ©
  ab-Î¸ (r- se) +á´¬ ab y
    âˆ
```


## Surjectivity

Every element of the abelian target is in the image of ab.

```agda
ab-surj : (a : Ab) â†’ Î£ Î» x â†’ ab x â‰¡ a
ab-surj (false , ğŸ¬) = E  , refl
ab-surj (false , ğŸ­) = R  , refl
ab-surj (false , ğŸ®) = RÂ² , refl
ab-surj (true  , ğŸ¬) = S  , refl
ab-surj (true  , ğŸ­) = SR , refl
ab-surj (true  , ğŸ®) = SRÂ² , refl
```


## Commutativity

The abelianization witnesses the commutativity of PSL2Z up to the
abelianization map.

```agda
ab-commutative : (x y : PSL2Z)
  â†’ ab (x Â· y) â‰¡ ab (y Â· x)
ab-commutative x y =
  ab-hom x y
  âˆ™ +á´¬-comm (ab x) (ab y)
  âˆ™ sym (ab-hom y x)
```
